%! app: TODOapp
%! outcome: TODOoutcome

{\bf Claim} $\forall s \in S \, (\textit{rnalen(s)} \geq \textit{basecount}(~(s, \A)~))$:

{\bf Proof}: We proceed by structural induction on the recursively defined set $S$.

{\bf Basis  Case}: We need to prove that 
the inequality holds for each element in the basis step of the recursive
definition of $S$. 
Need to show 
\begin{align*}
          &(~ rnalen(\A) \geq basecount(~(\A, \A)~)~) \land (~ rnalen(\C) \geq basecount(~(\C, \A)~)~) \\
    \land & (~ rnalen(\U) \geq basecount(~(\U, \A)~)~) \land (~ rnalen(\G) \geq basecount(~(\G, \A)~)~)
\end{align*}
We calculate, using the definitions of $rnalen$ and $basecount$:

\vspace{100pt}

{\bf Recursive Case}: We will prove that 
\[
    \forall u \in S ~\forall b \in B ~( ~rnalen(u) \geq basecount(~(u, \A)~) \to 
    rnalen(ub) \geq basecount(~(ub, \A)~)
\]

Consider arbitrary RNA strand $u$ and arbitrary base $b$. Assume, as the {\bf induction hypothesis},
that $rnalen(u) \geq basecount(~(u,\A)~)$. We need to show that $rnalen(ub) \geq basecount(~(ub, \A)~)$.

Using the recursive step in the definition of the function $rnalen$:
\[
    rnalen(ub) = 1 + rnalen(u)
\]
The recursive step in the definition of the function $basecount$ has two cases. We notice that 
$b = \A \lor b \neq \A$ and we proceed by cases.

{\it Case i.} Assume $b = \A$.

Using the first case in the recursive step in the definition of the function $basecount$:
\[
    basecount(~(ub, \A)~) = 1 + basecount(~(u,\A)~)
\]
By the {\bf induction hypothesis}, we know that $basecount(~(u,\A)~) \leq rnalen(u)$ so:
\[
    basecount(~(ub, \A)~) = 1 + basecount(~(u,\A)~) \leq 1 + rnalen(u) = rnalen (ub)
\]
and, thus, $basecount(~(ub,\A)~) \leq rnalen(ub)$, as required.

{\it Case ii.} Assume $b \neq \A$. 

Using the second case in the recursive step in the definition of the function $basecount$:
\[
    basecount(~(ub, \A)~) = basecount(~(u,\A)~)
\]
By the {\bf induction hypothesis}, we know that $basecount(~(u,\A)~) \leq rnalen(u)$ so:
\[
    basecount(~(ub, \A)~) = basecount(~(u,\A)~) \leq rnalen(u) < 1 + rnalen(u) = rnalen (ub)
\]
and, thus, $basecount(~(ub,\A)~) \leq rnalen(ub)$, as required.
